com.io7m.calino.specification/src/main/coq/Calino/Flag.v
@@ -1,13 +1,28 @@
 Require Import Coq.Strings.String.
+Require Import Coq.Lists.List.
+Require Import Coq.Unicode.Utf8_core.
 
 Require Import Calino.Descriptor.
 
+Import ListNotations.
+
 Inductive flag : Set :=
   | FlagAlphaPremultiplied
-  | FlagCustom : descriptor -> flag.
+  | FlagCustom : descriptor → flag.
 
 Definition flagDescribe (f : flag) : descriptor :=
   match f with
   | FlagAlphaPremultiplied => "ALPHA_PREMULTIPLIED"
   | FlagCustom d           => d
   end.
+
+#[export]
+Instance flagDescribable : describable flag := {
+  descriptorOf f := flagDescribe f
+}.
+
+Inductive flagSet : Set := {
+  flags      : list flag;
+  flagsNoDup : NoDup flags;
+}.
+
