com.io7m.calino.specification/src/main/coq/Calino/Binary.v
@@ -1,0 +1,343 @@
+Require Import Coq.Arith.PeanoNat.
+Require Import Coq.Strings.String.
+Require Import Coq.Lists.List.
+Require Import Coq.Init.Nat.
+Require Import Coq.Init.Byte.
+Require Import Coq.Bool.Bool.
+Require Import Coq.Program.Basics.
+Require Import Coq.Unicode.Utf8_core.
+
+Require Import Calino.Metadata.
+Require Import Calino.MipMap.
+Require Import Calino.ImageInfo.
+Require Import Calino.Divisible8.
+Require Import Calino.StringUtility.
+Require Import Calino.Descriptor.
+Require Import Calino.ChannelDescription.
+Require Import Calino.ChannelSemantic.
+Require Import Calino.ChannelType.
+Require Import Calino.Compression.
+Require Import Calino.SuperCompression.
+Require Import Calino.ColorSpace.
+Require Import Calino.Flag.
+Require Import Calino.ByteOrder.
+Require Import Calino.CoordinateSystem.
+Require Import Calino.ImageSize.
+
+Import ListNotations.
+
+Open Scope program_scope.
+Open Scope string_scope.
+
+Set Mangle Names.
+
+Inductive streamE : Set :=
+  | Vu64 : nat → streamE
+  | Vu32 : nat → streamE
+  | Vu8  : nat → streamE.
+
+Definition streamSize (s : streamE) : nat :=
+  match s with
+  | Vu64 _ => 8
+  | Vu32 _ => 4
+  | Vu8  _ => 1
+  end.
+
+Section binaryExpressions.
+
+  Local Unset Elimination Schemes.
+
+  Inductive binaryExp : Set :=
+    | BiU32     : nat → binaryExp
+    | BiU64     : nat → binaryExp
+    | BiBytes   : list byte → binaryExp
+    | BiUTF8    : list byte → binaryExp
+    | BiArray   : list binaryExp → binaryExp
+    | BiReserve : nat → binaryExp
+    | BiRecord  : list (string * binaryExp) → binaryExp.
+
+  Section binaryExp_rect.
+    Variable P             : binaryExp → Type.
+    Variable P_list        : list binaryExp → Type.
+    Hypothesis P_nil       : P_list [].
+    Hypothesis P_cons      : ∀ x xs, P x → P_list xs → P_list (x :: xs).
+    Hypothesis P_BiU32     : ∀ x, P (BiU32 x).
+    Hypothesis P_BiU64     : ∀ x, P (BiU64 x).
+    Hypothesis P_BiBytes   : ∀ bs, P (BiBytes bs).
+    Hypothesis P_BiUTF8    : ∀ bs, P (BiUTF8 bs).
+    Hypothesis P_BiArray   : ∀ bs, P_list bs → P (BiArray bs).
+    Hypothesis P_BiReserve : ∀ x, P (BiReserve x).
+    Hypothesis P_BiRecord  : ∀ fs, P_list (map snd fs) → P (BiRecord fs).
+
+    Fixpoint binaryExp_rect (b : binaryExp) : P b :=
+      let
+        fix expForAll (xs : list binaryExp) : P_list xs :=
+          match xs as rxs return (P_list rxs) with
+          | []        => @P_nil
+          | (y :: ys) => @P_cons y ys (binaryExp_rect y) (expForAll ys)
+          end
+      in let
+        fix forAllSnd (fs : list (string * binaryExp)) : P_list (map snd fs) :=
+          match fs as rf return P_list (map snd rf) with
+          | []             => @P_nil
+          | ((_, y) :: ys) => @P_cons y (map snd ys) (binaryExp_rect y) (forAllSnd ys)
+          end
+      in
+        match b with
+        | BiU32 c     => P_BiU32 c
+        | BiU64 c     => P_BiU64 c
+        | BiBytes bs  => P_BiBytes bs
+        | BiUTF8 bs   => P_BiUTF8 bs
+        | BiArray es  => P_BiArray es (expForAll es)
+        | BiReserve c => P_BiReserve c
+        | BiRecord fs => P_BiRecord fs (forAllSnd fs)
+        end.
+
+  End binaryExp_rect.
+
+  Section binaryExp_ind.
+    Variable P             : binaryExp → Prop.
+    Hypothesis P_BiU32     : ∀ x, P (BiU32 x).
+    Hypothesis P_BiU64     : ∀ x, P (BiU64 x).
+    Hypothesis P_BiBytes   : ∀ bs, P (BiBytes bs).
+    Hypothesis P_BiUTF8    : ∀ bs, P (BiUTF8 bs).
+    Hypothesis P_BiArray   : ∀ bs, Forall P bs → P (BiArray bs).
+    Hypothesis P_BiReserve : ∀ x, P (BiReserve x).
+    Hypothesis P_BiRecord  : ∀ fs, Forall P (map snd fs) → P (BiRecord fs).
+
+    Definition binaryExp_ind (b : binaryExp) : P b :=
+      binaryExp_rect 
+        P
+        (List.Forall P)
+        (List.Forall_nil _)
+        (λ x xs Px Pxs, List.Forall_cons _ Px Pxs)
+        P_BiU32
+        P_BiU64
+        P_BiBytes
+        P_BiUTF8
+        P_BiArray
+        P_BiReserve
+        P_BiRecord
+        b.
+
+  End binaryExp_ind.
+End binaryExpressions.
+
+Definition sizeMultipleOf (size q : nat) (Hnz : 0 ≠ q) : nat :=
+  let r := size / q in
+    match Nat.ltb_spec0 r q with
+    | ReflectT _ _ => (r + 1) * q
+    | ReflectF _ _ => r * q
+    end.
+
+Lemma p0not4 : 0 ≠ 4.
+Proof. discriminate. Qed.
+Lemma p0not16 : 0 ≠ 16.
+Proof. discriminate. Qed.
+
+Fixpoint binarySize (b : binaryExp) : nat :=
+  match b with
+  | BiU32 _     => 4
+  | BiU64 _     => 8
+  | BiBytes s   => 4 + sizeMultipleOf (length s) 4 p0not4
+  | BiUTF8 s    => 4 + sizeMultipleOf (length s) 4 p0not4
+  | BiArray f   => 4 + fold_right plus 0 (map binarySize f)
+  | BiReserve s => sizeMultipleOf s 4 p0not4
+  | BiRecord f  => fold_right plus 0 (map (binarySize ∘ snd) f)
+  end.
+
+Definition binaryEvalPaddedBytes 
+  (b     : list byte) 
+  (align : nat) 
+  (Hneq  : 0 ≠ align) 
+: list streamE :=
+  let v8 := map (Vu8 ∘ Byte.to_nat) b in
+  let vm := length v8 mod align in
+    match (Nat.eqb_spec 0 vm) with
+    | ReflectT _ _ => v8
+    | ReflectF _ _ => v8 ++ (repeat (Vu8 0) vm) 
+    end.
+
+Fixpoint binaryEval (b : binaryExp) : list streamE :=
+  match b with
+  | BiU32 k     => [Vu32 k]
+  | BiU64 k     => [Vu64 k]
+  | BiBytes s   => (Vu32 (length s)) :: (binaryEvalPaddedBytes s 4 p0not4)
+  | BiUTF8 s    => (Vu32 (length s)) :: (binaryEvalPaddedBytes s 4 p0not4)
+  | BiArray f   => fold_right (@app streamE) [] (map binaryEval f)
+  | BiReserve s => repeat (Vu8 0) (sizeMultipleOf s 4 p0not4)
+  | BiRecord f  => fold_right (@app streamE) [] (map (binaryEval ∘ snd) f)
+  end.
+
+Definition binarySizePadded16 (b : binaryExp) : nat :=
+  sizeMultipleOf (binarySize b) 16 p0not16.
+
+Definition utf8 (s : string) : binaryExp :=
+  BiUTF8 (list_byte_of_string s).
+
+Definition u32 := BiU32.
+Definition u64 := BiU64.
+
+Definition binaryExpMipMap (m : mipMap) : binaryExp := BiRecord [
+  ("mipMapLevel",            u32 (mipMapLevel m));
+  ("mipMapDataOffset",       u64 (mipMapOffset m));
+  ("mipMapSizeUncompressed", u64 (mipMapSizeUncompressed m));
+  ("mipMapSizeCompressed",   u64 (mipMapSizeCompressed m));
+  ("mipMapCRC32",            u32 (mipMapCRC32 m))
+].
+
+Definition binaryExpMipMaps (m : mipMapList) : binaryExp :=
+  BiArray (map binaryExpMipMap (mipMaps m)).
+
+Definition binaryExpCompression (c : compressionMethod) : binaryExp := BiRecord [
+  ("descriptor",        utf8 (descriptorOf c));
+  ("sectionIdentifier", u64 (compressionSectionIdentifier c));
+  ("blockSizeX",        u32 (compressionBlockSizeX c));
+  ("blockSizeY",        u32 (compressionBlockSizeY c));
+  ("blockAlignment",    u32 (compressionBlockAlignment c))
+].
+
+Definition binaryExpSuperCompression (c : superCompressionMethod) : binaryExp := BiRecord [
+  ("descriptor",        utf8 (descriptorOf c));
+  ("sectionIdentifier", u64 (superCompressionSectionIdentifier c))
+].
+
+Definition binaryExpImageInfo (i : imageInfo) : binaryExp := BiRecord [
+  ("sizeX",            u32 (imageSizeX i));
+  ("sizeY",            u32 (imageSizeY i));
+  ("sizeZ",            u32 (imageSizeZ i));
+  ("channelsLayout",   utf8 (descriptorOf (imageChannelsLayout i)));
+  ("channelsType",     utf8 (descriptorOf (imageChannelsType i)));
+  ("compression",      binaryExpCompression (imageCompressionMethod i));
+  ("superCompression", binaryExpSuperCompression (imageSuperCompressionMethod i));
+  ("coordinateSystem", utf8 (descriptorOf (imageCoordinateSystem i)));
+  ("colorSpace",       utf8 (descriptorOf (imageColorSpace i)));
+  ("flags",            BiArray (map (utf8 ∘ descriptorOf) (imageFlagSet i)));
+  ("byteOrder",        utf8 (descriptorOf (imageByteOrder i)))
+].
+
+Definition binaryExpFileHeader : binaryExp := BiRecord [
+  ("id",           u64 0x89434C4E0D0A1A0A);
+  ("versionMajor", u32 1);
+  ("versionMinor", u32 0)
+].
+
+Definition binaryExpImageInfoSection (i : imageInfo) : binaryExp := BiRecord [
+  ("id",   u64 0x434C4E49494E464F);
+  ("size", u64 (binarySizePadded16 (binaryExpImageInfo i)));
+  ("data", binaryExpImageInfo i)
+].
+
+Definition binaryExpMetadataValue (m : metadataValue) : binaryExp := BiRecord [
+  ("key",   utf8 (mKey m));
+  ("value", utf8 (mValue m))
+].
+
+Definition binaryExpMetadata (m : metadata) : binaryExp :=
+  BiArray (map binaryExpMetadataValue (mValues m)).
+
+Definition binaryExpMetadataSection (m : metadata) : binaryExp := BiRecord [
+  ("id",   u64 0x434C4E49494E464F);
+  ("size", u64 (binarySizePadded16 (binaryExpMetadata m)));
+  ("data", binaryExpMetadata m)
+].
+
+Definition binaryEndSection : binaryExp := BiRecord [
+  ("id",   u64 0x434c4e5f454e4421);
+  ("size", u64 0)
+].
+
+Lemma sizeMultipleOfMod : ∀ s q (Hneq : 0 ≠ q), (sizeMultipleOf s q Hneq) mod q = 0.
+Proof.
+  intros s q Hneq.
+  unfold sizeMultipleOf.
+  destruct (Nat.ltb_spec0 (s / q) q) as [Hlt|H1].
+  - apply (Nat.mod_mul (s / q + 1) q (Nat.neq_sym _ _ Hneq)).
+  - apply (Nat.mod_mul (s / q) q (Nat.neq_sym _ _ Hneq)).
+Qed.
+
+Lemma fold_right_add_cons : ∀ x xs,
+  x + fold_right plus 0 xs = fold_right plus 0 (x :: xs).
+Proof. reflexivity. Qed.
+
+Lemma forall_map_binarySize : ∀ es, 
+  Forall (λ b : binaryExp, binarySize b mod 4 = 0) es 
+    ↔ Forall (λ n, n mod 4 = 0) (map binarySize es).
+Proof.
+  intros es.
+  induction es.
+  constructor.
+  - rewrite Forall_map.
+    intros H. trivial.
+  - rewrite Forall_map.
+    intros H. trivial.
+  - rewrite Forall_map.
+    constructor.
+    intros H; trivial.
+    intros H; trivial.
+Qed.
+
+Theorem binarySizeMultiple4 : ∀ b, binarySize (b) mod 4 = 0.
+Proof.
+  intros b.
+  induction b as [Hbu32|Hbu64|Hbbyte|Hbutf|xs HFA|Hbuns|xs HFF] using binaryExp_ind.
+  (* U32 values are of size 4 *)
+  - reflexivity.
+  (* U64 values are of size 8 *)
+  - reflexivity.
+  (* Byte array values are rounded up to a multiple of 4 and prefixed with 4 *)
+  - unfold binarySize.
+    remember (sizeMultipleOf (Datatypes.length Hbbyte) 4 p0not4) as size eqn:Heqsize.
+    rewrite Nat.add_comm.
+    rewrite <- (Nat.add_mod_idemp_l size 4 4 (Nat.neq_sym _ _ p0not4)).
+    assert (size mod 4 = 0) as Hm0. {
+      rewrite Heqsize.
+      apply (sizeMultipleOfMod (Datatypes.length Hbbyte) 4 (p0not4)).
+    }
+    rewrite Hm0.
+    reflexivity.
+  (* UTF-8 values are rounded up to a multiple of 4 and prefixed with 4 *)
+  - unfold binarySize.
+    remember (sizeMultipleOf (Datatypes.length Hbutf) 4 p0not4) as size eqn:Heqsize.
+    rewrite Nat.add_comm.
+    rewrite <- (Nat.add_mod_idemp_l size 4 4 (Nat.neq_sym _ _ p0not4)).
+    assert (size mod 4 = 0) as Hm0. {
+      rewrite Heqsize.
+      apply (sizeMultipleOfMod (Datatypes.length Hbutf) 4 (p0not4)).
+    }
+    rewrite Hm0.
+    reflexivity.
+  (* Each element of an array is a multiple of 4, so the entire array is too. *)
+  - unfold binarySize.
+    fold binarySize.
+    induction xs as [|y ys HforAllInd].
+    -- reflexivity.
+    -- assert (fold_right add 0 (map binarySize (y :: ys)) mod 4 = 0) as HfoldEq. {
+         apply (@divisibilityNFoldPlus 4 (map binarySize (y :: ys))).
+         discriminate.
+         rewrite <- forall_map_binarySize.
+         exact HFA.
+       }
+       rewrite map_cons.
+       rewrite map_cons in HfoldEq.
+       assert (4 mod 4 = 0) as H4mod40 by (reflexivity).
+       assert (0 ≠ 4) as H0n4 by (discriminate).
+       apply (divisiblityNAdd 4 (fold_right add 0 (binarySize y :: map binarySize ys)) 4 H0n4 H4mod40 HfoldEq).
+  (* Unspecified values are rounded up. *)
+  - unfold binarySize.
+    rewrite sizeMultipleOfMod.
+    reflexivity.
+  (* Each element of an record is a multiple of 4, so the entire record is too. *)
+  - unfold binarySize.
+    fold binarySize.
+    induction xs as [|y ys HforAllInd].
+    -- reflexivity.
+    -- rewrite map_cons.
+       rewrite map_cons in HFF.
+       rewrite <- fold_right_add_cons.
+       apply divisiblityNAdd.
+       discriminate.
+       apply (Forall_inv HFF).
+       apply HforAllInd.
+       apply (Forall_inv_tail HFF).
+Qed.
