com.io7m.calino.specification/src/main/coq/Calino/ColorSpace.v
@@ -1,11 +1,12 @@
 Require Import Coq.Strings.String.
+Require Import Coq.Unicode.Utf8_core.
 
 Require Import Calino.Descriptor.
 
 Inductive colorSpace : Set :=
   | CSLinear
   | CSsRGB
-  | CSCustom : descriptor -> colorSpace.
+  | CSCustom : descriptor → colorSpace.
 
 Definition colorSpaceDescribe (c : colorSpace) : descriptor :=
   match c with
@@ -18,3 +19,4 @@ Definition colorSpaceDescribe (c : colorSpace) : descriptor :=
 Instance colorSpaceDescribable : describable colorSpace := {
   descriptorOf c := colorSpaceDescribe c
 }.
+
