com.io7m.calino.specification/src/main/coq/Calino/Divisible8.v
@@ -1,30 +1,62 @@
 Require Import Coq.PArith.PArith.
 Require Import Coq.Arith.PeanoNat.
 Require Import Coq.Init.Nat.
+Require Import Coq.Lists.List.
 Require Import Coq.Unicode.Utf8_core.
 
-Set Mangle Names.
+(* Set Mangle Names. *)
 
 Definition divisible8 (x : nat) : Prop :=
   modulo x 8 = 0.
+
+Theorem divisiblityNAdd : ∀ (x y z : nat),
+  0 ≠ z → x mod z = 0 → y mod z = 0 → (x + y) mod z = 0.
+Proof.
+  intros x y z Hz Hx Hy.
+  destruct y as [|y].
+    (* If y = 0, then this matches one of our assumptions already. *)
+    rewrite Nat.add_0_r; exact Hx.
+    (* Otherwise, the following property always holds given that the divisor is ≠ 0. *)
+    assert ((x mod z + S y) mod z = (x + S y) mod z) as Heq.
+      apply (Nat.add_mod_idemp_l x (S y) z).
+      apply (Nat.neq_sym 0 z Hz).
+    (* x mod z = 0 *)
+    rewrite Hx in Heq.
+    (* 0 + S y = S y *)
+    rewrite Nat.add_0_l in Heq.
+    rewrite <- Heq.
+    exact Hy.
+Qed.
+
+Theorem divisibilityNFoldPlus : ∀ z xs,
+  0 ≠ z →
+    Forall (λ n, n mod z = 0) xs →
+      (fold_right plus 0 xs) mod z = 0.
+Proof.
+  intros z xs Hnz HforAll.
+  induction xs as [|y ys].
+  - apply (Nat.mod_0_l z (Nat.neq_sym 0 z Hnz)).
+  - assert (fold_right add 0 (y :: ys) = y + fold_right add 0 ys) as Hfoldeq by reflexivity.
+    rewrite Hfoldeq.
+    assert (fold_right add 0 ys mod z = 0) as Hfoldeq2. {
+      apply IHys.
+      apply (@Forall_inv_tail nat (λ n : nat, n mod z = 0) y ys HforAll).
+    }
+    rewrite divisiblityNAdd.
+    reflexivity.
+    exact Hnz.
+    apply (@Forall_inv nat (λ n : nat, n mod z = 0) y ys HforAll).
+    exact Hfoldeq2.
+Qed.
 
 Theorem divisiblity8Add : ∀ (x y : nat),
   divisible8 x → divisible8 y → divisible8 (x + y).
 Proof.
   intros x y Hx Hy.
   unfold divisible8 in *.
-  destruct y as [|y].
-    (* If y = 0, then this matches one of our assumptions already. *)
-    rewrite Nat.add_0_r; exact Hx.
-    (* Otherwise, the following property always holds given that the divisor is 8. *)
-    assert ((x mod 8 + S y) mod 8 = (x + S y) mod 8) as Heq.
-      apply (Nat.add_mod_idemp_l x (S y) 8).
-      discriminate.
-    (* x mod 8 = 0 *)
-    rewrite Hx in Heq.
-    (* 0 + S y = S y *)
-    rewrite Nat.add_0_l in Heq.
-    rewrite <- Heq.
-    exact Hy.
+  apply divisiblityNAdd.
+  discriminate.
+  trivial.
+  trivial.
 Qed.
 
