com.io7m.calino.specification/src/main/coq/Calino/ImageSize.v
@@ -1,0 +1,11 @@
+Require Import Coq.Unicode.Utf8_core.
+
+Record imageSize3D : Set := ImageSize3D {
+  sizeX     : nat;
+  sizeY     : nat;
+  sizeZ     : nat;
+  sizeXnot0 : 0 ≠ sizeX;
+  sizeYnot0 : 0 ≠ sizeY;
+  sizeZnot0 : 0 ≠ sizeZ;
+}.
+
