com.io7m.calino.specification/src/main/coq/Calino/Metadata.v
@@ -1,0 +1,16 @@
+Require Import Coq.Strings.String.
+Require Import Coq.Strings.Ascii.
+Require Import Coq.Lists.List.
+Require Import Coq.Unicode.Utf8_core.
+
+Open Scope string_scope.
+
+Inductive metadataValue : Set := MetadataValue {
+  mKey   : string;
+  mValue : string
+}.
+
+Inductive metadata : Set := Metadata {
+  mValues : list metadataValue
+}.
+
