com.io7m.calino.specification/src/main/coq/Calino/MipMap.v
@@ -1,4 +1,10 @@
+Require Import Coq.Arith.PeanoNat.
 Require Import Coq.Lists.List.
+Require Import Coq.Init.Nat.
+Require Import Coq.Bool.Bool.
+Require Import Coq.Unicode.Utf8_core.
+
+Require Import Calino.ImageSize.
 
 Import ListNotations.
 
@@ -10,15 +16,68 @@ Inductive mipMap : Set := MipMap {
   mipMapCRC32            : nat
 }.
 
-Inductive mipMapListIsSorted : list mipMap -> Prop :=
-  | MipsOne   : forall m, mipMapListIsSorted [m]
-  | MipsCons  : forall mm0 mm1 mxs, 
-    mipMapLevel mm1 = S (mipMapLevel mm0) ->
-      mipMapListIsSorted (mm0 :: mxs) ->
+Inductive mipMapListIsSorted : list mipMap → Prop :=
+  | MipsOne   : ∀ m, mipMapListIsSorted [m]
+  | MipsCons  : ∀ mm0 mm1 mxs,
+    mipMapLevel mm1 = S (mipMapLevel mm0) →
+      mipMapListIsSorted (mm0 :: mxs) →
         mipMapListIsSorted (mm1 :: mm0 :: mxs).
 
 Inductive mipMapList : Set := MipMapList {
-  mipMaps            : list mipMap;
-  mipMapListNonEmpty : nil <> mipMaps;
-  mipMapListSorted   : mipMapListIsSorted mipMaps
+  mipMaps          : list mipMap;
+  mipMapListSorted : mipMapListIsSorted mipMaps
 }.
+
+Inductive mipMapImageSize : Set := MipMapImageSize {
+  mmSizeX      : nat;
+  mmSizeY      : nat;
+  mmSizeZ      : nat;
+  mmSizeXRange : 1 < mmSizeX;
+  mmSizeYRange : 1 < mmSizeY;
+  mmSizeZRange : 0 < mmSizeZ;
+}.
+
+Lemma lt_neq : ∀ n, 0 ≠ n ↔ 0 < n.
+Proof.
+  intros n.
+  constructor.
+  - intro Hneq.
+    induction n as [|k].
+    -- unfold not in Hneq.
+       assert (0 = 0) as Heq by reflexivity.
+       contradiction.
+    -- apply (Nat.lt_0_succ k).
+  - intro Hneq.
+    induction n as [|k].
+    -- inversion Hneq.
+    -- discriminate.
+Qed.
+
+Lemma lt_neq_0 : ∀ n, 0 ≠ n → 0 < n.
+Proof.
+  intros n Hneq.
+  rewrite <- lt_neq; trivial.
+Qed.
+
+Lemma lt_neq_1 : ∀ n, 0 < n → 0 ≠ n.
+Proof.
+  intros n Hneq.
+  rewrite lt_neq; trivial.
+Qed.
+
+Definition mipMapSize 
+  (level      : nat) 
+  (imageSize  : imageSize3D)
+  (levelRange : 0 < level)
+: option mipMapImageSize :=
+  let sx := (sizeX imageSize) / 2 ^ level in
+  let sy := (sizeY imageSize) / 2 ^ level in
+    match (Nat.ltb_spec0 1 sx, Nat.ltb_spec0 1 sy) with
+    | (ReflectT _ xt, ReflectT _ yt) =>
+      let z  := sizeZ imageSize in
+      let zn := lt_neq_0 z (sizeZnot0 imageSize) in
+        Some (MipMapImageSize sx sy z xt yt zn)
+    | (_, _) => 
+      None
+    end.
+
