com.io7m.calino.specification/src/main/coq/Calino/SuperCompression.v
@@ -1,11 +1,12 @@
 Require Import Coq.Strings.String.
+Require Import Coq.Unicode.Utf8_core.
 
 Require Import Calino.Descriptor.
 
 Inductive superCompressionMethod : Set :=
   | SuperCompressionUncompressed
   | SuperCompressionLZ4
-  | SuperCompressionCustom : descriptor -> nat -> superCompressionMethod.
+  | SuperCompressionCustom : descriptor → nat → superCompressionMethod.
 
 Definition superCompressionMethodDescriptor (c : superCompressionMethod) :=
   match c with
@@ -20,7 +21,15 @@ Definition superCompressionIsNotCompressed (c : superCompressionMethod) : Prop :
   | _                            => False
   end.
 
+Definition superCompressionSectionIdentifier (c : superCompressionMethod) : nat :=
+  match c with
+  | SuperCompressionUncompressed => 0
+  | SuperCompressionLZ4          => 0
+  | SuperCompressionCustom _ i   => i
+  end.
+
 #[export]
 Instance superCompressionMethodDescribable : describable superCompressionMethod := {
   descriptorOf c := superCompressionMethodDescriptor c
 }.
+
