com.io7m.calino.specification/src/main/coq/make.sh
@@ -2,6 +2,7 @@
 
 coqc -Q Calino Calino Calino/StringUtility.v
 coqc -Q Calino Calino Calino/Divisible8.v
+coqc -Q Calino Calino Calino/Metadata.v
 coqc -Q Calino Calino Calino/Descriptor.v
 coqc -Q Calino Calino Calino/ChannelSemantic.v
 coqc -Q Calino Calino Calino/ChannelDescription.v
@@ -12,9 +13,11 @@ coqc -Q Calino Calino Calino/ColorSpace.v
 coqc -Q Calino Calino Calino/ByteOrder.v
 coqc -Q Calino Calino Calino/Flag.v
 coqc -Q Calino Calino Calino/CoordinateSystem.v
+coqc -Q Calino Calino Calino/ImageSize.v
 coqc -Q Calino Calino Calino/ImageInfo.v
 coqc -Q Calino Calino Calino/MipMap.v
 coqc -Q Calino Calino Calino/Image.v
+coqc -Q Calino Calino Calino/Binary.v
 
 mkdir -p html
 
